Lp2lc/Active/STLC/Sanity.lean
@@ -13,6 +13,7 @@ def denotation : (self : Trm TrmVar) -> self.Denotation :=
   fun self =>
     match self with
     | .var name declared => .var name declared
+    | .literal instructions declared => .literal instructions declared
     | .function body => .function body
     | .apply fn arg => .apply (denotation fn) (denotation arg)
 
@@ -24,6 +25,78 @@ namespace Sanity
 
 -- All docstrings use short (under 5 lines) of Scala code as demonstrations.
 
+abbrev base_variable : Trm Unit :=
+  Trm.var () .base
+
+abbrev arrow_variable : Trm Unit :=
+  Trm.var () (.base :=> .base)
+
+abbrev one_argument_base_function : Trm Unit :=
+  Trm.function (fun argument => .var argument .base)
+
+abbrev applies_to_base_variable : Trm Unit :=
+  Trm.apply one_argument_base_function base_variable
+
+abbrev applies_to_arrow_variable : Trm Unit :=
+  Trm.apply one_argument_base_function arrow_variable
+
+abbrev invalid_application : Trm Unit :=
+  Trm.apply base_variable base_variable
+
+example : Typ.base.AsSemantic (TrmVar := Unit) base_variable = True := by
+  apply propext
+  constructor
+  · intro _
+    trivial
+  · intro _
+    simpa [base_variable] using
+      (Typ.AsSemantic.var (name := ()) (declared := Typ.base))
+
+example : Typ.base.AsSemantic (TrmVar := Unit) applies_to_base_variable = True := by
+  apply propext
+  constructor
+  · intro _
+    trivial
+  · intro _
+    unfold applies_to_base_variable one_argument_base_function base_variable
+    refine Typ.AsSemantic.apply (tIn := Typ.base) ?_ ?_
+    · refine Typ.AsSemantic.function ?_
+      intro argument
+      exact Typ.AsSemantic.var
+    · exact Typ.AsSemantic.var
+
+example : Typ.base.AsSemantic (TrmVar := Unit) applies_to_arrow_variable = True := by
+  apply propext
+  constructor
+  · intro _
+    trivial
+  · intro _
+    unfold applies_to_arrow_variable one_argument_base_function arrow_variable
+    refine Typ.AsSemantic.apply (tIn := Typ.base :=> Typ.base) ?_ ?_
+    · refine Typ.AsSemantic.function ?_
+      intro argument
+      exact Typ.AsSemantic.var
+    · exact Typ.AsSemantic.var
+
+example : Typ.base.AsSemantic (TrmVar := Unit) one_argument_base_function = False := by
+  apply propext
+  constructor
+  · intro typing
+    unfold one_argument_base_function at typing
+    cases typing
+  · intro falsehood
+    cases falsehood
+
+example : Typ.base.AsSemantic (TrmVar := Unit) invalid_application = False := by
+  apply propext
+  constructor
+  · intro typing
+    unfold invalid_application base_variable at typing
+    cases typing with
+    | apply function_typing _ =>
+        cases function_typing
+  · intro falsehood
+    cases falsehood
 
 
 end Sanity
